adding initial res_to_copland translator skeleton

src/Resolute_Logic.v
@@ -1,68 +1,115 @@
-(* Encoding of the RESOLUTE logic in coq *)
+(* Encoding of the RESOLUTE logic (and RESOLUTE to Copland translator) in coq *)
 
-Require Export String.
+Require Export String Maps OptMonad_Coq.
 Require Export List.
 
-(*
-Inductive Formula : Type :=
-  | false
-  | true
-  | Var : string -> Formula
-  | Not : Formula -> Formula
-  | Impl : Formula -> Formula -> Formula.
-*)
+(* Generic ID Type -- for now, just make it nat *)
+Definition ID_Type := nat.
 
-(*
-Inductive FinTypeElems : Set := 
-| FinType1_Elems
-| FinType2_Elems.
-*)
+(* Target ID *)
+Definition Target_ID := ID_Type.
+(* Target Group ID -- some meaningful (but abstract) grouping of targets *)
+Definition Target_Group := ID_Type.
+(* A concrete set of targets *)
+Definition Target_Pool := list Target_ID.
 
+(* ASP (Attestation Service Provider) IDs *)
+Definition ASP_ID := ID_Type.
 
-Definition FinSet : Set.  Admitted.
-(*
-Inductive FinSet : Set :=
-| Threads
-| Memories.
+(* Explicit mapping from target groups to pools *)
+Definition Target_Map := MapC Target_Group Target_Pool.
 
-Inductive FixedThreadPool : Set := 
-| Thread1
-| Thread2
-| ThreadBob.
-*)
+(* Explicit mapping from target IDs to the ASP IDs that measure those targets *)
+Definition Measures_Map := MapC Target_ID ASP_ID.
 
+Inductive Term : Type := 
+| emptyTerm : Term
+| aspTerm : ASP_ID -> Term
+| seqTerm : Term -> Term -> Term.
 
-Definition FinSetElements (T:FinSet) : Set.  Admitted.
-(*
-Definition FinSetElements (T:FinSet) : Set :=
-  match T with
-  | Threads => FixedThreadPool
-  | Memories => list nat
+Inductive Evidence : Type := 
+| emptyE : Evidence
+| aspE : ASP_ID -> Evidence
+| seqE : Evidence -> Evidence -> Evidence.
+
+Inductive AppEvidence : Type := 
+| app_emptyE : AppEvidence
+| app_aspE : ASP_ID -> AppEvidence 
+| app_seqE : AppEvidence -> AppEvidence -> AppEvidence.
+
+(* Abstract system measurement -- vastly simplified simulation 
+   of the Copland Virtual Machine (CVM) *)
+Fixpoint measure (t:Term) : Evidence := 
+  match t with 
+  | emptyTerm => emptyE
+  | aspTerm i => aspE i 
+  | seqTerm t1 t2 => seqE (measure t1) (measure t2)
   end.
-*)
+
+(* Abstract appraisal procedure *)
+Fixpoint appraise (e:Evidence) : AppEvidence := 
+  match e with
+  | emptyE => app_emptyE
+  | aspE i => app_aspE i 
+  | seqE e1 e2 => app_seqE (appraise e1) (appraise e2)
+  end.
+
+(* This will probably need more parameters going forward...
+   something like a "cert strategy"... *)
+Definition cert_policy (appE:AppEvidence) : bool.
+Admitted.
+
+Definition end_to_end_cert (t:Term) : bool :=
+  cert_policy (appraise (measure t)).
 
 Inductive Resolute : Type :=
   | R_False
   | R_True
-  | R_Goal (T : FinSet)
+  | R_Goal (T : Target_ID)
   | R_And (G1 : Resolute) (G2 : Resolute)
   | R_Or (G1 : Resolute) (G2 : Resolute)
   | R_Imp (G1 : Resolute) (G2 : Resolute)
-  | R_Forall (T: FinSet) (G : (FinSetElements T) -> Resolute)
-  | R_Exists (T : FinSet) (G : (FinSetElements T) -> Resolute).
+  | R_Forall (T : Target_Group)  (G : Target_ID -> Resolute)
+  | R_Exists (T : Target_Group) (G : Target_ID -> Resolute).
 
 Definition Assumption := Resolute.
 Definition Assumptions := list (Assumption).
 
-(*
-Inductive Reval : Assumptions -> Resolute -> Prop :=
-  | eval_L (A : Assumptions) (e : Assumption) (G : Resolute) :
-    e = R_Goal false -> Reval (e::A) G
-  | eval_R (A : Assumptions) (G : Resolute) :
-    G = R_Goal true -> Reval A G
-  | R_And_eval (A : Assumptions) (G1 G2 : Resolute) : 
-    Reval A G1 -> Reval A G2 -> Reval A (R_And G1 G2).
-*)
+(* Get all ASP_IDs of corresponding Target_IDs in Measures_Map *)
+Definition get_aspids (ls:list Target_ID) (mm:Measures_Map) : Opt (list ASP_ID).
+Admitted.
+
+(* Construct a compound Term from a list of ASP_IDs *)
+Definition aspids_to_term (ls:list ASP_ID) : Term.
+Admitted.
+
+Fixpoint res_to_copland (r:Resolute) (mm:Measures_Map) (tm:Target_Map) : Opt Term :=
+  match r with 
+  | R_False => failm 
+  | R_True => ret emptyTerm
+  | (R_Goal tid) => 
+      i <- (map_get mm tid) ;;
+      (ret (aspTerm i))
+  | R_And r1 r2 => 
+    t1 <- res_to_copland r1 mm tm ;;
+    t2 <- res_to_copland r2 mm tm ;;
+    ret (seqTerm t1 t2)
+  | R_Or r1 r2 => 
+    t1 <- res_to_copland r1 mm tm ;;
+    t2 <- res_to_copland r2 mm tm ;;
+    ret (seqTerm t1 t2)
+  | R_Imp r1 r2 => 
+    res_to_copland r1 mm tm (* Is generating terms for antecedent enough here? *)
+  | R_Forall tg pred => 
+    pool <- map_get tm tg ;;
+    asp_ids <- (get_aspids pool mm) ;;
+    ret (aspids_to_term asp_ids)
+  | R_Exists tg pred => 
+    pool <- map_get tm tg ;;
+    asp_ids <- (get_aspids pool mm) ;;
+    ret (aspids_to_term asp_ids)
+  end.
+ 
 
 Inductive Reval : Assumptions -> Resolute -> Prop :=
   | Reval_L : forall A G,
@@ -77,23 +124,31 @@ Inductive Reval : Assumptions -> Resolute -> Prop :=
     (Reval A G2) -> Reval A (R_Or G1 G2)
   | Reval_Imp : forall A G1 G2,
     Reval (G1::A) G2 -> Reval A (R_Imp G1 G2)
-  | Reval_Forall{T:FinSet} : forall (A:Assumptions) (pred: (FinSetElements T) -> Resolute),      
-      (forall (v:FinSetElements T), Reval A (pred v)) ->
-      Reval A (R_Forall T pred)
-  | Reval_Exists{T:FinSet} : forall (A:Assumptions) (pred: (FinSetElements T) -> Resolute),
-      (exists (v:FinSetElements T), Reval A (pred v)) -> 
-      Reval A (R_Exists T pred).
-    (*
-  | Reval_Forall_nil : forall A G,
-    Reval A (R_Forall nil G)
-  | Reval_Forall : forall A n ns G,
-    Reval A (G n) -> Reval A (R_Forall ns G) -> Reval A (R_Forall (n::ns) G)
-    
-  | Reval_Exists_skip : forall A n ns G,
-    Reval A (R_Exists ns G) -> Reval A (R_Exists (n::ns) G)
-  | Reval_Exists : forall A n ns G,
-    Reval A (G n) -> Reval A (R_Exists (n::ns) G).
-    *)
+  | Reval_Forall : forall (A:Assumptions) (m:Target_Map) 
+    (gr:Target_Group) (tp:Target_Pool) (pred: Target_ID -> Resolute),      
+      (forall (v:Target_ID), 
+        map_get m gr = Some tp -> 
+        In v tp -> 
+        Reval A (pred v)) ->
+      Reval A (R_Forall gr pred)
+  | Reval_Exists : forall (A:Assumptions) (m:Target_Map) 
+    (gr:Target_Group) (tp:Target_Pool) (pred: Target_ID -> Resolute),      
+      (exists (v:Target_ID), 
+        map_get m gr = Some tp -> 
+        In v tp -> 
+        Reval A (pred v)) ->
+      Reval A (R_Exists gr pred).
+
+
+Theorem res_to_copland_sound : forall (a:Assumptions) (r:Resolute) mm tm, 
+  (exists t, 
+    (res_to_copland r mm tm = Some t) /\ 
+  end_to_end_cert t = true) 
+  <->
+  Reval a r.
+Proof.
+Admitted.
+
 
 Example test_RAnd :
   Reval ((R_And (R_False) (R_True))::nil) (R_And (R_False) (R_True)).
@@ -115,6 +170,9 @@ Proof.
   apply Reval_Imp. apply Reval_R.
 Qed.
 
+
+
+(*
 Example test_RForall :
   Reval (nil) (R_Forall (5 :: (2 :: (3 :: nil))) (R_Goal)).
 Proof.
@@ -129,3 +187,4 @@ Example test_RExists :
 Proof.
   apply Reval_Exists_skip. apply Reval_Exists. admit.
 Admitted.
+*)
